---
{"dg-publish":true,"dg-permalink":"数学/每日一题/260","permalink":"/数学/每日一题/260/","dgHomeLink":true,"dgPassFrontmatter":false}
---


![](https://mmbiz.qpic.cn/mmbiz_jpg/QVficiaYicXqN1GHlpTdbiaPl3BD7ux3FFKCXCMichrib7uCoI9SP9TVNiaWrQsIXHwTqgAFIz21GeVm6JZoOnOterC9Q/640?wx_fmt=jpeg&wxfrom=5&wx_lazy=1&wx_co=1)

```ad-ans
collapse:true

C.
$$
\begin{align}
\lim_{ x \to 1 } \left( \frac{f(x)-2x}{e^{x-1}-1}-\frac{1}{\ln x} \right)&=\lim_{ x \to 1 } \frac{\ln x(f(x)-2x)-(e^{x-1}-1)}{(x-1)^{2} }\\
&=\lim_{ x \to 1 } \frac{\left( \left( (x-1)-\frac{1}{2}(x-1)^{2} \right)(f(1)-2)-\left( (x-1)+\frac{1}{2}(x-1)^{2} \right) \right)}{(x-1)^{2} }\\
&=-\frac{1}{2}(f(1)-2)-\frac{1}{2}\\
f(x)-2&=1\\
f(x)&=3
\end{align}
$$
```

