---
{"dg-publish":true,"dg-permalink":"数学/每日一题/268","permalink":"/数学/每日一题/268/","dgHomeLink":true,"dgPassFrontmatter":false}
---

![](https://mmbiz.qpic.cn/mmbiz_png/QVficiaYicXqN07CPscziafpjjyibVRTu8yqpdc5fibau3NLdG1ic7Mmoibo1hKBAl19Y4jNLwFt7QCzoCFA9PW5STeJ4A/640?wx_fmt=png&wxfrom=5&wx_lazy=1&wx_co=1)

```ad-ans
collapse:true
$$
\begin{align}
\lim_{ x \to 1 } \left( \sqrt{ \frac{(1+x^{2})\sqrt{ x }}{e^{x-1}} }+\arctan\frac{x^{2}-1}{\sqrt{ 1+x^{2} }}+1-\sqrt{ 2 } \right)^{\frac{1}{\ln x}}&=\lim_{ x \to 1 }\exp\frac{\sqrt{ \frac{(1+x^{2})\sqrt{ x }}{e^{x-1}} }+\arctan\frac{x^{2}-1}{\sqrt{ 1+x^{2} }}-\sqrt{ 2 }}{x-1}\\
&=\lim_{ x \to 1 } \exp\frac{ \sqrt{ 2 }\left( \sqrt{\frac{ (1+x^{2})\sqrt{ x } }{2e^{x-1}}} -1 \right)+\arctan \frac{x^{2}-1}{\sqrt{ 1+x^{2} }}}{x-1}\\
&=\lim_{ x \to 1 } \exp \frac{\frac{\sqrt{ 2 }}{2}\left( \frac{(1+x^{2})\sqrt{ x }}{2e^{x-1}}-1 \right)+\frac{x^{2}-1}{\sqrt{ 1+x^{2} }}}{x-1}\\
&=\exp \left( \lim_{ x \to 1 } \frac{\sqrt{ 2 }}{2}\frac{ \ln\left( \frac{1+x^{2}}{2} \right)+\frac{1}{2}\ln(x)-x+1}{x-1}+\sqrt{ 2 } \right)\\
&=\exp\left(\frac{\sqrt{ 2 }}{2}\left(1+\frac{1}{2}-1 \right)+\sqrt{ 2 }\right)\\
&=e^{\frac{5\sqrt{ 2 }}{4}}
\end{align}
$$
```
