---
{"dg-publish":true,"dg-permalink":"数学/不定积分/不定积分题集","permalink":"/数学/不定积分/不定积分题集/","dgHomeLink":true,"dgPassFrontmatter":false}
---


1. $$
\int \frac{-x^{2}-2}{(x^{2}+x+1)^{2} } \, \mathrm{d}x 
$$
```ad-ans
collapse:true
$$
\begin{align}
\int \frac{-x^{2}-2}{(x^{2}+x+1)^{2} } \, \mathrm{d}x &=\int -\frac{1}{x^{2}+x+1} \, \mathrm{d}x+\int \frac{x+\frac{1}{2} } {(x^{2}+x+1)^{2} } \, \mathrm{d}x  +\int -\frac{3}{2} \frac{1}{(x^{2}+x+1)^{2} } \, \mathrm{d}x  \\
&=\int -\frac{1}{\left( x+\frac{1}{2} \right)^{2}+\frac{3}{4} } \, \mathrm{d}x +\int \frac{1}{2} \frac{1}{(x^{2}+x+1)^{2} }  \, \mathrm{d}(x^{2}+x+1)+\int -\frac{3}{2} \frac{1}{(x^{2}+x+1)^{2} }  \, \mathrm{d}x \\
&=-\frac{2}{\sqrt{ 3 } }\arctan \frac{2x+1}{\sqrt{ 3 } }-\frac{1}{2} \frac{1}{x^{2}+x+1}- \frac{3}{2} \int \frac{1}{(x^{2}+x+1)^{2} }  \, \mathrm{d}x  \\
 \int \frac{1}{(x^{2}+x+1)^{2} }  \, \mathrm{d}x &\xlongequal{\frac{2}{\sqrt{ 3 } }\left( x+\frac{1}{2} \right)=\tan u}\int \frac{1}{\frac{3}{4}( \tan ^{2}u +1)^{2} } \, \mathrm{d}\left( \frac{\sqrt{ 3 } }{2}\tan u-\frac{1}{2} \right)  \\
&=\frac{8}{3\sqrt{ 3 } }\int \frac{\sec ^{2}u}{\sec^4u} \, \mathrm{d}u \\
&=\frac{8}{3\sqrt{ 3 } }\int \cos ^{2}u \, \mathrm{d}u   \\
&=\frac{8}{3\sqrt{ 3 } }\int \frac{\cos 2u+1}{2} \, \mathrm{d}u \\
&=\frac{2}{3\sqrt{ 3 } }\sin 2u+\frac{4}{3\sqrt{ 3 } }u+C \\
&=\frac{2}{3\sqrt{ 3 } } \frac{\frac{4}{\sqrt{ 3 } }\left( x+\frac{1}{2} \right)}{1+\frac{4}{3}\left( x+\frac{1}{2} \right)^{2} } + \frac{4}{3\sqrt{ 3 } }\arctan \frac{2x+1}{\sqrt{ 3 } } +C\\
原式&=-\frac{4}{\sqrt{ 3 } }\arctan\frac{2x+1}{\sqrt{ 3 } }-\frac{x+1}{x^{2}+x+1}+C
\end{align}
$$
```

2. $$\int \frac{\mathrm{d}x}{\sqrt[3]{ (x+1)^{2}(x-1)^{4} } } $$
```ad-ans
collapse:true
$$\begin{align}
\int \frac{\mathrm{d}x}{\sqrt[3]{ (x+1)^{2}(x-1)^{4} } } &=\int \frac{\mathrm{d}x}{(x-1)^{2}\sqrt[3]{\left( \frac{x+1}{x-1} \right)^{2}  } } \\
&=-\int \frac{1}{\sqrt[3]{\left( \frac{x+1}{x-1} \right)^{2}  } } \, \mathrm{d}\left( \frac{1}{x-1} \right) \\
&\xlongequal{u=\frac{1}{x-1} }-\int \frac{1}{\sqrt[3]{(1+2u)^{2}  } } \, \mathrm{d}u \\
&=-\frac{3}{2}\sqrt[3]{(1+2u)^{2} }+C \\
&=-\frac{3}{2}\sqrt[3]{\left( \frac{x+1}{x-1} \right)^{2}  }+C  
\end{align}
$$
```

3. $$\int e^{ax}\cos bx \, \mathrm{d}x $$
```ad-ans
collapse:true
分类讨论，切切切！
$$\begin{align} \\
a\neq0,\\
\int e^{ax}\cos bx \, \mathrm{d}x &= \frac{1}{a}e^{ax}\cos bx+\frac{b}{a}\int   e^{ax}\sin bx \,\mathrm{d}x  \\
&=\frac{1}{a}e^{ax}\cos bx+\frac{b}{a^{2} }e^{ax}\sin bx-\frac{b^{2} }{a^{2} }\int e^{ax}\cos bx \, \mathrm{d}x  \\
\Rightarrow \int e^{ax}\cos bx \, \mathrm{d}x&=\frac{a\cos bx+b\sin bx}{a^{2}+b^{2} }e^{ax}+C \\
a=0, \\
\int e^{ax}\cos bx \, \mathrm{d}x&=\int \cos bx  \, \mathrm{d}x =\frac{1}{b}\sin bx+C
\end{align}
$$
```

4. $$\int \frac{\sin ^{2}x}{\cos ^{3}x} \, \mathrm{d}x $$
```ad-ans
collapse:true
$$\begin{align}
\int \frac{\sin ^{2}x}{\cos ^{3}x} \, \mathrm{d}x&=\int \sec^{3}x \, \mathrm{d}x-\int \sec x \, \mathrm{d}x   \\
\int \sec ^{3}x \, \mathrm{d}x&=\int \tan x \, \mathrm{d}\sec x+\int \sec x \, \mathrm{d}x    \\
&=\tan x\sec x+\int \sec x \, \mathrm{d}x -\int \sec ^{3} \, \mathrm{d}x  \\
\Rightarrow \int \sec ^{3}x \, \mathrm{d}x &=\frac{1}{2}\tan x\sec x+\frac{1}{2}\int \sec x \, \mathrm{d}x \\
原式&=\frac{1}{2}\tan x\sec x-\frac{1}{2}\ln|\sec x+\tan x|+C
\end{align}$$
```

5. $$\int \arctan \sqrt{ x } \, \mathrm{d}x $$
```ad-ans
collapse:true
$$\begin{align}
\int \arctan \sqrt{ x } \, \mathrm{d}x &= \int \arctan \sqrt{ x } \, \mathrm{d}(x+1)\\
&=(x+1)\arctan x-\frac{1}{2}\int \frac{1}{\sqrt{ x } } \, \mathrm{d}x \\
&=(x+1)\arctan x-\sqrt{ x }+C
\end{align}$$
```

6. $$\int \frac{\sqrt{ 1+\cos x } }{\sin x} \, \mathrm{d}x $$
```ad-ans
collapse:true
分类讨论切切切！
$$\begin{align}
\int \frac{\sqrt{ 1+\cos x } }{\sin x} \, \mathrm{d}x &= \int \frac{1}{\sqrt{ 2 } } \frac{|\cos \frac{x}{2}|}{\cos \frac{x}{2}\sin \frac{x}{2} } \, \mathrm{d}x \\
x\in\left(4k\pi-\pi,4k\pi+\pi\right),\quad&=\frac{1}{\sqrt{ 2 } }\csc \frac{x}{2}dx=\sqrt{ 2 }
\ln\left|\csc \frac{x}{2}-\cot \frac{x}{2}\right|+C\\
&=\sqrt{ 2 }\ln\frac{1-\cos \frac{x}{2} }{|\sin \frac{x}{2}|}+C\\
&=\sqrt{ 2 }\ln\left( \left|\csc \frac{x}{2}\right|-|\cot \frac{x}{2}| \right)+C\\
x\in\left(4k\pi-\pi,4k\pi+\pi\right),\quad&=-\frac{1}{\sqrt{ 2 } }\csc \frac{x}{2}dx=-\sqrt{ 2 }\ln\left|\csc \frac{x}{2}-\cot \frac{x}{2}\right|+C\\
&=-\sqrt{ 2 }\ln\frac{1-\cos \frac{x}{2} }{|\sin \frac{x}{2}|}+C\\
&=-\sqrt{ 2 }\ln\left(\left|\csc \frac{x}{2}\right| +\left|\csc \frac{x}{2}\right|\right)+C\\
&=\sqrt{ 2 }\ln\left( \left|\csc \frac{x}{2}\right|-|\cot \frac{x}{2}| \right)+C\end{align}$$

```

7. $$
\int \frac{x+\sin x}{1+\cos x} \, \mathrm{d}x 
$$
```ad-ans
collapse:true

消干净，切切切！
$$\begin{align}
\int \frac{x+\sin x}{1+\cos x} \, \mathrm{d}x&=\int \frac{x}{2\cos ^{2} \frac{x}{2} } \, \mathrm{d}x -\ln(1+\cos x)\\
&\xlongequal{u=\frac{x}{2} }2\int u\sec ^{2}u \, \mathrm{d}u-\ln(1+\cos x)\\
&=2u\tan u-2\int \tan u \, \mathrm{d}u-\ln(1+\cos x)\\
&=x\tan \frac{x}{2}+\textcolor{red}{2\ln|\cos \frac{x}{2}|-\ln(1+\cos x)}+C\\
&=x\tan \frac{x}{2}+C
\end{align}$$
```

8. $$
\int \frac{e^{3x}+e^{x} }{e^{4x}-e^{2x}+1} \, \mathrm{d}x 
$$
```ad-ans
collapse:true

注意次数，切切切！！
$$
\begin{align}
\int \frac{e^{3x}+e^{x} }{e^{4x}-e^{2x}+1} \, \mathrm{d}x &= \int \frac{e^{x}+e^{-x} }{e^{2x}-1+e^{-2x} } \, \mathrm{d}x \\
&\xlongequal{u=e^{x}-e^{-x} }\int \frac{1}{u^{2}+1} \, \mathrm{d}u\\
&=\arctan(e^{x}-e^{-x})+C
\end{align}
$$
```

9. $$
\int \frac{\ln x}{(1+x^{2})^{\frac{3}{2} }} \, \mathrm{d}x 
$$

```ad-ans
collapse:true

$$
\begin{align}
\int \frac{\ln x}{(1+x^{2})^{\frac{3}{2} }} \, \mathrm{d}x&=\int \ln x \, \mathrm{d}\left( -\frac{x}{\sqrt{1+x^{2} }} \right)\\
&=-\frac{x\ln x}{\sqrt{ 1+x^{2} } }+\int \frac{1}{\sqrt{ 1+x^{2} } } \, \mathrm{d}x\\
&=-\frac{x\ln x}{\sqrt{ 1+x^{2} } }+\ln\left|x+\sqrt{ 1+x^{2} }\right|+C
\end{align}
$$
or$\bigstar$
$$
\begin{align}
\int \frac{\ln x}{(1+x^{2})^{\frac{3}{2} }} \, \mathrm{d}x&\xlongequal{u=\frac{1}{x} }\int \frac{u\ln u}{(1+u^{2})^{\frac{3}{2} }} \, \mathrm{d}u\\
&=-\frac{\ln u}{\sqrt{ 1+u^{2} } }+\int \frac{\mathrm{d}u}{u\sqrt{ 1+u^{2} } }\\
&=\frac{x\ln x}{\sqrt{ 1+x^{2} } }-\ln\left(x+\sqrt{ 1+x^{2} }\right)+C
\end{align}
$$
```

10. $$
\int \sqrt{ 1-x^{2} }\arcsin x \, \mathrm{d}x 
$$
```ad-ans
collapse:true

$$
\begin{align}
\int \sqrt{ 1-x^{2} }\arcsin x \, \mathrm{d}x &\xlongequal{u=\arcsin x,u\in\left( -\frac{\pi}{2},\frac{\pi}{2} \right)}\int u\cos ^{2} u \, \mathrm{d}x\\
&=\frac{1}{2}\int u(\cos 2u+1) \, \mathrm{d}x\\
&=\frac{1}{8}\int 2u(\cos 2u+1) \, \mathrm{d}(2u)\\
&=\frac{1}{4}u^{2}+\frac{1}{4}u\sin 2u-\frac{1}{8}\cos 2u+C\\
&=\frac{1}{4}\arctan ^{2}x+\frac{1}{2}x\sqrt{ 1-x^{2} }\arcsin x+\frac{1}{4}x^{2}+C
\end{align} 
$$
```

11. $$
\int \frac{\cot x}{1+\sin x} \, \mathrm{d}x 
$$
```ad-ans
collapse:true
$$
\begin{align}
\int \frac{\cot x}{1+\sin x} \, \mathrm{d}x &=\int \frac{1}{\sin x(1+\sin x)} \, \mathrm{d}\sin x\\
&=\ln|\sin x|-\ln(1+\sin x)+C
\end{align}
$$

```

12. $$
\int \frac{\mathrm{d}x}{\sin ^{3}x\cos x}
$$
```ad-ans
collapse:true
$$
\begin{align}
\int \frac{\mathrm{d}x}{\sin ^{3}x\cos x}&=\int \cot x\sec^{2} x \, \mathrm{d}(\cot x)\\
&\xlongequal{u=\cot x}-\int u\left( 1+ \frac{1}{u^{2} } \right) \, \mathrm{d}u\\
&=-\frac{u^{2} }{2}-\ln|u|+C\\
&=-\frac{\cot ^{2}x}{2}-\ln|\cot x|+C
\end{align}
$$
```

13. $$
\int \frac{\sin x\cos x}{\sin x+\cos x} \, \mathrm{d}x 
$$

```ad-ans
collapse:true
$$
\begin{align}
\int \frac{\sin x\cos x}{\sin x+\cos x} \, \mathrm{d}x &=\int \frac{\sin x\cos x}{2\sqrt{ 2 }\sin\left( x+\frac{\pi}{4} \right)}\, \mathrm{d}x \\
&\xlongequal{u=x+\frac{\pi}{4} }\int \frac{2\sin ^{2}u-1}{2\sqrt{ 2 }\sin u} \, \mathrm{d}u \\
&=\frac{1}{\sqrt{ 2 } }\int \sin u \, \mathrm{d}u-\frac{1}{2\sqrt{ 2 } }\int \csc u \, \mathrm{d}u  \\
&=-\frac{\cos\left( x+\frac{\pi}{4} \right)}{\sqrt{ 2 } }-\frac{1}{2\sqrt{ 2 } }\ln\left|\csc\left( x+\frac{\pi}{4} \right)-\cot\left( x+\frac{\pi}{4} \right)\right|+C
\end{align}
$$
```

14. $$
\int \frac{\sin 2x}{\sqrt{ a^{2}\sin ^{2}x+b^{2}\cos ^{2}x }} \, \mathrm{d}x\quad(|a|\neq|b|) 
$$
```ad-ans
collapse:true
$$
\begin{align}
(a^{2}\sin ^{2}x+b^{2}\cos ^{2}x)'&=^{2}a\sin 2x-b^{2}\sin 2x\\
\int \frac{\sin 2x}{\sqrt{ a^{2}\sin ^{2}x+b^{2}\cos ^{2}x }} \, \mathrm{d}x&=\int \frac{1}{a^{2}-b^{2}} \frac{1}{\sqrt{ a^{2}\sin ^{2}x+b^{2}\cos ^{2}x }} \, \mathrm{d}(a^{2}\sin ^{2}x+b^{2}\cos ^{2}x)\\
&=\frac{2}{a^{2}-b^{2}}\sqrt{ a^{2}\sin ^{2} x+b^{2}\cos ^{2}x }+C
\end{align}
$$

```

15. $$
\int \frac{x}{\sqrt{ 1+x^{2}+(1+x^{2})\sqrt{ 1+x^{2} } }} \, \mathrm{d}x 
$$
```ad-ans
collapse:true
$$
\begin{align}
\int \frac{x}{\sqrt{ 1+x^{2}+(1+x^{2})\sqrt{ 1+x^{2} } }} \, \mathrm{d}x &=\frac{1}{2}\int \frac{\mathrm{d}(x^{2}+1)}{\sqrt{ 1+x^{2} }\sqrt{ 1+\sqrt{ 1+x^{2} } }}\\
&=\int \frac{\mathrm{d}(\sqrt{ 1+x^{2} }+1)}{\sqrt{ 1+\sqrt{ 1+x^{2} } }}\\
&=2\sqrt{ 1+\sqrt{ 1+x^{2} } }+C
\end{align}$$

```

16. $$
\begin{align}
&\text{设}f(x)\text{为单调函数},\text{且}\int f(x) \, \mathrm{d}x =F(x)+C,\text{则}\int f^{-1}(x) \, \mathrm{d}x= (\ \ )
\\&A.F^{-1}(x)+C
\\&B.xf^{-1}(x)-F[f^{-1}(x)]+C
\\&C.F[f^{-1}(x)]+C
\\&D.xf^{-1}(x)+C
\end{align}
$$

```ad-ans
collapse:true

B.
$$
\begin{align}
\int f^{-1}(x) \, \mathrm{d}x &=xf^{-1}(x)-\int x \, \mathrm{d}(f^{-1}(x)) \\
&=xf^{-1}(x)-\int f(f^{-1}(x)) \, \mathrm{d}(f^{-1}(x)) 
\end{align}
$$
```

17. $$
\int \frac{1}{x}\sqrt{ \frac{1+x}{1-x} } \, \mathrm{d}x 
$$

```ad-ans
collapse:true
$$
\begin{align}
\int \frac{1}{x}\sqrt{ \frac{1+x}{1-x} } \, \mathrm{d}x &=\int \frac{1}{\sqrt{ 1-x^{2} }} \, \mathrm{d}x +\int \frac{1}{x\sqrt{ 1-x^{2} }} \, \mathrm{d}x\\
&=\arcsin x-\int \frac{1}{\sqrt{ \frac{1}{x^{2}}-1 }} \, \mathrm{d}\frac{1}{x} \\
&=\arcsin x-\ln\left| \frac{1}{x}+\sqrt{ \frac{1}{x^{2}}-1 }\right|+C
\end{align}
$$
```

