---
{"dg-publish":true,"dg-permalink":"数学/微分方程/一阶线性微分方程","permalink":"/数学/微分方程/一阶线性微分方程/","dgHomeLink":true,"dgPassFrontmatter":false}
---


# 线性方程
- 一般形式$$\frac{ \mathrm{d}y }{ \mathrm{d}x } +P(x)y=Q(x)$$
- 对应齐次线性方程$\frac{ \mathrm{d}y }{ \mathrm{d}x } +P(x)y=0$的通解$$y=Ce^{-\int P(x) \, \mathrm{d}x }$$
- 常数变易法$C\implies u(x)$，得非齐次线性方程通解$$
y=e^{-\int P(x) \, \mathrm{d}x }\left( \int Q(x)e^{\int P(x) \, \mathrm{d}x } \, \mathrm{d}x +C \right)
$$

# 伯努利方程
- 一般形式$$\frac{ \mathrm{d}y }{ \mathrm{d}x } +P(x)y=Q(x)y^{n}\quad(n\neq 0,n\neq 1)$$
- 解法
	- 化为$$y^{-n}\frac{ \mathrm{d}y }{ \mathrm{d}x } +P(x)y^{1-n}=Q(x)$$
		- 令$z=y^{1-n}$，则$\frac{ \mathrm{d}z }{ \mathrm{d}x } =(1-n)y^{-n}\frac{ \mathrm{d}y }{ \mathrm{d}x }$，原方程化为$$\frac{ \mathrm{d}z }{ \mathrm{d}x } +(1-n)P(x)z=(1-n)Q(x)$$
